hack away at commutativity-strategy

examples/concurrency-strategies/commutativity-strategy.dfy
@@ -1,8 +1,251 @@
 include "spec.s.dfy"
 
+module Concrete {
+  import Abstract
+  import opened Options
+
+  datatype Well = Well(stones: nat)
+
+  datatype Thread = Thread(lockHeld: nat, victim:nat)
+    // Thread's goal is to find a well containing victim stones, and add a stone to it.
+
+  type Board = seq<Well>
+
+  datatype State = State(board:Board, threads:map<int, Thread>)
+
+  function View(board:Board, i:nat) : (v:seq<nat>)
+    requires 0 <= i <= |board|
+    ensures |v| == |board| - i
+    ensures forall j | 0<=j<|v| :: v[j] == board[j+i].stones
+    decreases |board| - i
+  {
+    if i < |board| then
+      [board[i].stones] + View(board, i+1)
+    else
+      []
+  }
+ 
+  function {:opaque} MapRemove1<K,V>(m:map<K,V>, k:K) : (m':map<K,V>)
+    ensures forall j :: j in m && j != k ==> j in m'
+    ensures forall j :: j in m' ==> j in m && j != k
+    ensures forall j :: j in m' ==> m'[j] == m[j]
+    ensures |m'.Keys| <= |m.Keys|
+    ensures k in m ==> |m'| == |m| - 1
+    ensures k !in m ==> |m'| == |m|
+  {
+    var m' := map j | j in m && j != k :: m[j];
+    assert m'.Keys == m.Keys - {k};
+    m'
+  }
+
+  predicate Init(s: State) {
+    && (forall i | 0 <= i < |s.board| :: s.board[i].stones == 0)  // not necessary, just feels right
+    && s.threads == map[]
+  }
+
+  predicate LockFree(s: State, lockId:nat) {
+    forall t: Thread | t in s.threads.Values :: t.lockHeld != lockId
+  }
+
+  predicate Start(s: State, s':State, victim:nat, tid: int, ui:Abstract.UI) {
+    var newThread := Thread(0, victim);
+    && LockFree(s, 0)
+    && s'.board == s.board
+    && tid !in s.threads
+    && s'.threads == s.threads[tid := newThread]
+    && ui == None
+    && s'.board == s.board
+  }
+
+  predicate Advance(s: State, s':State, tid: int, ui:Abstract.UI) {
+    && tid in s.threads
+    && var t := s.threads[tid];
+    && var nextLock := t.lockHeld + 1;
+    && 0 <= t.lockHeld < |s.board|
+    && if s.board[t.lockHeld].stones == t.victim then
+      // yay we found it!
+      && s'.board == s.board[t.lockHeld := s.board[t.lockHeld].(stones := t.victim + 1)]
+      // we're done! exit the runnable queue
+      && s'.threads == MapRemove1(s.threads, tid)
+      && ui == Some(Abstract.DonateOp(t.victim, Some(t.lockHeld)))
+    else if |s.board| <= nextLock then
+      // Ran off end of list without finding victim.
+      && s'.board == s.board
+      // we're done! exit the runnable queue
+      && s'.threads == MapRemove1(s.threads, tid)
+      && ui == Some(Abstract.DonateOp(t.victim, None))
+    else if LockFree(s, nextLock) then
+      var t' := Thread(nextLock, t.victim);
+      && s'.board == s.board
+      && s'.threads == s.threads[tid := t']
+      && ui == None
+    else
+      // Need to advance, but waiting on a lock
+      && s' == s
+      && ui == None
+  }
+
+  predicate Next(s:State, s':State, tid: int, ui:Abstract.UI) {
+    || (exists victim :: Start(s, s', victim, tid, ui))
+    || Advance(s, s', tid, ui)
+  }
+}
+
+module ConcreteOrdered {
+  import Concrete
+  import Abstract
+  import opened Options
+
+  datatype Variables = Variables(
+      state: Concrete.State,
+      orders: map<int, int>
+  )
+
+  predicate Next(s: Variables, s': Variables, tid: int, ui:Abstract.UI, my_rank: int)
+  {
+    && Concrete.Next(s.state, s'.state, tid, ui)
+    && (tid !in s.state.threads && tid in s'.state.threads ==>
+      s'.orders == s.orders[tid := my_rank]
+    )
+    && (tid in s.state.threads && tid !in s'.state.threads ==>
+      && s'.orders == Concrete.MapRemove1(s.orders, tid)
+    )
+    && (tid !in s.state.threads && tid !in s'.state.threads ==>
+      && s'.orders == s.orders
+    )
+    && (tid in s.state.threads && tid in s'.state.threads ==>
+      && tid in s.orders
+      && s.orders[tid] == my_rank
+      && s'.orders == s.orders
+    )
+  }
+
+  predicate ThreadsOrdered(s: Variables, tid1: int, tid2: int)
+  {
+    tid1 in s.orders && tid2 in s.orders && s.orders[tid1] < s.orders[tid2] ==>
+      && tid1 in s.state.threads
+      && tid2 in s.state.threads
+      && s.state.threads[tid1].lockHeld < s.state.threads[tid2].lockHeld
+  }
+
+  predicate LocksDistinct(s: Variables, tid1: int, tid2: int)
+  {
+    tid1 in s.state.threads && tid2 in s.state.threads && tid1 != tid2 ==>
+        s.state.threads[tid1].lockHeld != s.state.threads[tid2].lockHeld
+  }
+
+  predicate Inv(s: Variables)
+  {
+    && (forall tid1, tid2 :: ThreadsOrdered(s, tid1, tid2))
+    && (forall tid1, tid2 :: LocksDistinct(s, tid1, tid2))
+  }
+
+  lemma Commute(s: Variables, s1: Variables, s12: Variables,
+      tid1: int, ui1: Abstract.UI, my_rank1: int,
+      tid2: int, ui2: Abstract.UI, my_rank2: int)
+  returns (s2: Variables)
+  requires Inv(s)
+  requires Inv(s1)
+  requires Inv(s12)
+  requires Next(s, s1, tid1, ui1, my_rank1)
+  requires Next(s1, s12, tid2, ui2, my_rank2)
+  requires my_rank1 > my_rank2
+  requires tid1 != tid2
+  requires !(
+      && tid1 in s1.state.threads && s1.state.threads[tid1].lockHeld == 0
+      && tid2 in s12.state.threads && s12.state.threads[tid2].lockHeld == 0
+    )
+  ensures Next(s, s2, tid2, ui2, my_rank2)
+  ensures Next(s2, s12, tid1, ui1, my_rank1)
+  {
+    assert ThreadsOrdered(s, tid2, tid1);
+    assert LocksDistinct(s, tid1, tid2);
+
+    if Concrete.Advance(s1.state, s12.state, tid2, ui2) {
+      var t := s.state.threads[tid2];
+      assert t == s1.state.threads[tid2];
+      assert s.state.board[t.lockHeld] == s1.state.board[t.lockHeld];
+
+      var nextLock := t.lockHeld + 1;
+      if s.state.board[t.lockHeld].stones == t.victim {
+        // yay we found it!
+        var board := s.state.board[t.lockHeld := s.state.board[t.lockHeld].(stones := t.victim + 1)];
+        var threads := Concrete.MapRemove1(s.state.threads, tid2);
+        var orders := Concrete.MapRemove1(s.orders, tid2);
+        s2 := Variables(Concrete.State(board, threads), orders);
+
+        assert ui2.Some?;
+        assert ui2.value.victim == t.victim;
+        assert ui2.value.outidx == Some(t.lockHeld);
+        assert Concrete.Advance(s.state, s2.state, tid2, ui2);
+        assert Next(s, s2, tid2, ui2, my_rank2);
+      } else if |s.state.board| <= nextLock {
+        var board := s.state.board;
+        var threads := Concrete.MapRemove1(s.state.threads, tid2);
+        var orders := Concrete.MapRemove1(s.orders, tid2);
+        s2 := Variables(Concrete.State(board, threads), orders);
+
+        assert Next(s, s2, tid2, ui2, my_rank2);
+      } else if Concrete.LockFree(s.state, nextLock) {
+        var t' := Concrete.Thread(nextLock, t.victim);
+        var board := s.state.board;
+        var threads := s.state.threads[tid2 := t'];
+        var orders := s.orders;
+        s2 := Variables(Concrete.State(board, threads), orders);
+
+        assert Next(s, s2, tid2, ui2, my_rank2);
+      } else {
+        var board := s.state.board;
+        var threads := s.state.threads;
+        var orders := s.orders;
+        s2 := Variables(Concrete.State(board, threads), orders);
+
+        assert Next(s, s2, tid2, ui2, my_rank2);
+      }
+    } else {
+      var victim :| Concrete.Start(s1.state, s12.state, victim, tid2, ui2);
+      var board := s.state.board;
+      var newThread := Concrete.Thread(0, victim);
+      var threads := s.state.threads[tid2 := newThread];
+      var orders := s.orders[tid2 := my_rank2];
+      s2 := Variables(Concrete.State(board, threads), orders);
+
+      forall id | id in s.state.threads
+      ensures s.state.threads[id].lockHeld != 0
+      {
+        assert LocksDistinct(s, id, tid1);
+        assert LocksDistinct(s, id, tid2);
+        assert id != tid2;
+        if id == tid1 {
+          if s.state.threads[tid1].lockHeld == 0 {
+            assert ThreadsOrdered(s12, tid2, tid1);
+            assert tid1 in s1.state.threads;
+            assert s1.state.threads[tid1].lockHeld == 0;
+            assert tid2 in s12.state.threads;
+            assert s12.state.threads[tid2].lockHeld == 0;
+            assert false;
+          }
+          // Ordering is used here:
+          //assert s12.state.threads[tid1].lockHeld
+          //    > s12.state.threads[tid2].lockHeld;
+          //assert s1.state.threads[tid1].lockHeld
+          //    == s.state.threads[tid1].lockHeld;
+        } else {
+          assert s1.state.threads[id].lockHeld
+              == s.state.threads[id].lockHeld;
+        }
+      }
+      assert Concrete.Start(s.state, s2.state, victim, tid2, ui2);
+      assert Next(s, s2, tid2, ui2, my_rank2);
+    }
+
+    assert Next(s2, s12, tid1, ui1, my_rank1);
+  }
+}
+
 module TheoremProof {
 
-  lemma Correctness(b:Behavior<Concrete.State>, I:CState->AState)
+  /*lemma Correctness(b:Behavior<Concrete.State>, I:CState->AState)
     requires Reachable(b, Concrete.Init, Concrete.Next)
     ensures var ab := Interpret(b, I); Reachable(ab, Abstract.Init, Abstract.Next)
   {
@@ -24,7 +267,7 @@ module TheoremProof {
 
       assert Reachable(ab, Abstract.Init, Abstract.Next);
     }
-  }
+  }*/
   
 
 }
